%----------------------------------------------------------------------------------------
%	SECTION X.X
%----------------------------------------------------------------------------------------

\section{The Well Ordering Principle.}

\begin{enumerate}[label=(\arabic*)]
    \item [(2)]
        \begin{enumerate}
            \item $2^n=(1+1)^n=\sum {n \choose k}1^{n-k}1^k=\sum {n \choose k}$.

            \item $(a+b)^n=\sum_{k=0}^{n} {n \choose k}a^{n-k}b^k=a+na^{n-1}b+A$, hence $a+na^{n-1}b \leq (a+b)^n$

            \item $(1+\frac{1}{n})^n=\sum_{k=0}^{n} {n \choose k} \frac{1}{n^k} = 1+\frac{1}{n}+A=\frac{n+1}{n}+A$. Now since 
                $n \neq 0$, and  $n \in \N$, then  $n \geq 1$, so  $\frac{n+1}{n} \geq 2$, therefore so is $(1+\frac{1}{n})^n$
        \end{enumerate}

    \item [(3)]
        \begin{align*}
            \frac{(x+h)^n-x^n}{h} &= \frac{x^n-x^n+\sum_{k=0}^{n} {n \choose k} x^{n-k}h^k}{h} \\ 
                                  &= \frac{\sum {n \choose k} x^{n-k}k^k}{h} \\
                                  &= \sum_{k=2}^{n} {n \choose k} x^{n-k}h^{k-1} \\
        \end{align*}  

    \item [(5)] Since $0<x_1<2$, $x_1^2-x_1-2<0$, hence $x_1<\sqrt{2+x_1}=x_2$. Now suppose that for $n \geq 1$ that  
        $0<x_n<x_{n+1}<2$, and let  $k=n+2$. Then  $x_k=\sqrt{2+n_{n+1}}$ ; and we have that $x_{n+1}^2-x_{n+1}-2<0$, hence 
        $x_{n+1}<\sqrt{2+x_{n+1}}=x_k$. Therefore  $0<x_{n+1}<x_{n+2}<2$.

    \item  [(6)]
        \begin{enumerate}
            \item For $n=1$,  $1<2^1$. Now suppose for $n \geq 1$ that $n<2^n$, then $n+1<2^n+1<2^n+2^n=2^{n+1}$.

            \item For $n=1$, $1  \leq 2^1+1=3$. Now suppose that for $n \geq 1$ that $n^2 \leq 2^n+1$. Notice that for $n=2$ that 
                $2n+1>2^n$, so fo  $n \geq 3$ let $2n+1 < 2^n$, then $2n+1+2<2^n+2<2^n+2^n<2^{n+1}$ so $$. Notice then 
                $(n+1)^2=n^2+2n+1 \leq 2^n+1+2n+1 \leq 2^n+2^n+1 \leq 2^{n+1}+1$.

            \item For  $n=1$, then  $13<3^1$; now suppose for  $n \geq 1$ that  $(n+1)^3<3^n$. Then  $(n+1)^3=n^3+3n^2+3n+1<
                3^n+3n^2+3n+1<3^n+3^n+3^n=3^{n+1}$.
        \end{enumerate}
\end{enumerate}
